src/dafny/beacon/StateTransition.dfy
@@ -15,7 +15,10 @@
 include "../utils/Eth2Types.dfy"
 include "../utils/Helpers.dfy"
 include "../ssz/Constants.dfy"
+include "BeaconConstants.dfy"
 include "BeaconChain.dfy"
+include "../ssz/Eth2TypeDependentConstants.dfy"
+include "../merkle/Merkleise.dfy"
 
 /**
  * State transition function for the Beacon Chain.
@@ -27,93 +30,19 @@ module StateTransition {
     import opened Constants
     import opened BeaconChain
     import opened Helpers
+    import opened BeaconConstants
+    import opened Eth2TypeDependentConstants
+    import opened SSZ_Merkleise
 
-    /** The default zeroed Bytes32.  */
-    const SEQ_EMPTY_32_BYTES := timeSeq<byte>(0,32)
-    
-    /**
-     *  The default (empty) Bytes32
-     */
-    const EMPTY_BYTES32 : Bytes32 := Bytes(SEQ_EMPTY_32_BYTES)
 
-    /** The historical roots type.  */
-    const EMPTY_HIST_ROOTS := timeSeq<Bytes32>(EMPTY_BYTES32, SLOTS_PER_HISTORICAL_ROOT as int)
 
-    type VectorOfHistRoots = x : seq<Bytes32> |  |x| == SLOTS_PER_HISTORICAL_ROOT as int
-        witness EMPTY_HIST_ROOTS
 
-    /**
-     *  Compute Root/Hash/Bytes32 for different types.
-     *  
-     *  @todo   Use the hash_tree_root from Merkle.
-     */
-    function method hash_tree_root<T(==)>(t : T) : Bytes32 
-        ensures hash_tree_root(t) != EMPTY_BYTES32
-
-    /** Collision free hash function. 
-     *  This does not seem to affect the proofs so far, so
-     *  this lemma is commented out.
-     **/
-    // lemma {:axiom} foo<T(==)>(t1: T, t2: T) 
-        // ensures t1 == t2 <==> hash_tree_root(t1) == hash_tree_root(t2)
-
-   
-    /** 
-     * @link{https://notes.ethereum.org/@djrtwo/Bkn3zpwxB?type=view} 
-     * The beacon chain’s state (BeaconState) is the core object around 
-     * which the specification is built. The BeaconState encapsulates 
-     * all of the information pertaining to: 
-     *  - who the validators are, 
-     *  - in what state each of them is in, 
-     *  - which chain in the block tree this state belongs to, and 
-     *  - a hash-reference to the Ethereum 1 chain.
-
-     * Beginning with the genesis state, the post state of a block is 
-     * considered valid if it passes all of the guards within the state 
-     * transition function. Thus, the precondition of a block is 
-     * recursively defined as being a valid postcondition of running 
-     * the state transition function on the previous block and its state 
-     * all the way back to the genesis state.
-     *
-     * @param   slot                            Time is divided into “slots” of fixed length 
-     *                                          at which actions occur and state transitions 
-     *                                          happen. This field tracks the slot of the 
-     *                                          containing state, not necessarily the slot 
-     *                                          according to the local wall clock
-     * @param   latest_block_header             The latest block header seen in the chain 
-     *                                          defining this state. This blockheader has
-     *                                          During the slot transition 
-     *                                          of the block, the header is stored without the 
-     *                                          real state root but instead with a stub of Root
-     *                                          () (empty 0x00 bytes). At the start of the next 
-     *                                          slot transition before anything has been 
-     *                                          modified within state, the state root is 
-     *                                          calculated and added to the 
-     *                                          latest_block_header. This is done to eliminate 
-     *                                          the circular dependency of the state root 
-     *                                          being embedded in the block header
-     * @param   block_roots                     Per-slot store of the recent block roots. 
-     *                                          The block root for a slot is added at the start 
-     *                                          of the next slot to avoid the circular 
-     *                                          dependency due to the state root being embedded 
-     *                                          in the block. For slots that are skipped (no 
-     *                                          block in the chain for the given slot), the 
-     *                                          most recent block root in the chain prior to 
-     *                                          the current slot is stored for the skipped 
-     *                                          slot. When validators attest to a given slot, 
-     *                                          they use this store of block roots as an 
-     *                                          information source to cast their vote.
-     * @param   state_roots                     Per-slot store of the recent state roots. 
-     *                                          The state root for a slot is stored at the 
-     *                                          start of the next slot to avoid a circular 
-     *                                          dependency
-     */
-    datatype BeaconState = BeaconState(
-        slot: Slot,
-        latest_block_header: BeaconBlockHeader,
-        block_roots: VectorOfHistRoots,
-        state_roots: VectorOfHistRoots
-    )
+    function method castToBeaconState(s:RawSerialisable): BeaconState
+    requires s.BeaconState?
+    requires wellTypedContainer(s)
+    {
+        s
+    }    
 
     /**
      *  Whether a block is valid in a given state.
@@ -125,17 +54,17 @@ module StateTransition {
      */
     predicate isValid(s : BeaconState, b : BeaconBlockHeader) 
     {
-        s.slot < b.slot 
+        s.slot.n < b.slot.n
         //  Fast forward s to b.slot and check `b` can be attached to the
         //  resulting state's latest_block_header.
         && b.parent_root == 
-            hash_tree_root(
+            getHashTreeRootBytes32(
                 forwardStateToSlot(resolveStateRoot(s), 
-                b.slot
+                b.slot.n as Slot
             ).latest_block_header) 
-        &&  b.state_root == hash_tree_root(
+        &&  b.state_root == getHashTreeRootBytes32(
                 addBlockToState(
-                    forwardStateToSlot(resolveStateRoot(s), b.slot), 
+                    forwardStateToSlot(resolveStateRoot(s), b.slot.n as Slot), 
                     b
                 )
             )
@@ -152,17 +81,17 @@ module StateTransition {
         /** The next state latest_block_header is same as b except for state_root that is 0. */
         ensures s'.latest_block_header == b.(state_root := EMPTY_BYTES32)
         /** s' slot is now adjusted to the slot of b. */
-        ensures s'.slot == b.slot
+        ensures s'.slot.n == b.slot.n
         /** s' parent_root is the hash of the state obtained by resolving/forwarding s to
             the slot of b.  */
         ensures s'.latest_block_header.parent_root  == 
-            hash_tree_root(
-                forwardStateToSlot(resolveStateRoot(s), b.slot)
+            getHashTreeRootBytes32(
+                forwardStateToSlot(resolveStateRoot(s), b.slot.n as Slot)
                 .latest_block_header
             )
     {
         //  finalise slots before b.slot.
-        var s1 := processSlots(s, b.slot);
+        var s1 := processSlots(s, b.slot.n as Slot);
 
         //  Process block and compute the new state.
         s' := processBlock(s1, b);  
@@ -170,7 +99,7 @@ module StateTransition {
         // Verify state root (from eth2.0 specs)
         // A proof that this assert statement is never violated when isValid() is true.
         // if validate_result:
-        assert (b.state_root == hash_tree_root(s'));
+        assert (b.state_root == getHashTreeRootBytes32(s'));
 
     }  
 
@@ -202,19 +131,19 @@ module StateTransition {
      *                  resolveStateRoot(s); 
      *
      */
-    method processSlots(s: BeaconState, slot: Slot) returns (s' : BeaconState)
-        requires s.slot < slot  //  update in 0.12.0 (was <= before)
+    method {:fuel wellTypedContainer,2}  processSlots(s: BeaconState, slot: Slot) returns (s' : BeaconState)    
+        requires s.slot.n < slot as nat  //  update in 0.12.0 (was <= before)
 
         ensures s' == forwardStateToSlot( resolveStateRoot(s), slot)
         ensures s.latest_block_header.parent_root == s'.latest_block_header.parent_root  
         
         //  Termination ranking function
-        decreases slot - s.slot
+        decreases slot as nat - s.slot.n
     {
         //  Start from the current state and update it with processSlot.
         //  First iteration of the loop in process_slots (Eth2)
         s' := processSlot(s);
-        s':= s'.(slot := s'.slot + 1) ;
+        s':= castToBeaconState(s'.(slot := Uint64(s'.slot.n + 1))) ;
         //  The following asserts are not needed for the proof but provided for readability. 
         assert(s' == resolveStateRoot(s));  
         //  s'.block header state_root should now be resolved
@@ -222,20 +151,20 @@ module StateTransition {
 
         //  Now fast forward to slot
         //  Next iterations of process_slot (Eth2)
-        while (s'.slot < slot)  
-            invariant s'.slot <= slot
+        while (s'.slot.n < slot as nat) 
+            invariant s'.slot.n <= slot as nat
             invariant s'.latest_block_header.state_root != EMPTY_BYTES32
-            invariant s' == forwardStateToSlot(resolveStateRoot(s), s'.slot) // Inv1
-            decreases slot - s'.slot 
+            invariant s' == forwardStateToSlot(resolveStateRoot(s), s'.slot.n as Slot) // Inv1
+            decreases slot as nat - s'.slot.n
         {
             s':= processSlot(s');
 
             //  s'.slot is now processed: history updated and block header resolved
             //  The state's slot is processed and we can advance to the next slot.
-            s':= s'.(slot := s'.slot + 1) ;
+            s':= castToBeaconState(s'.(slot := Uint64(s'.slot.n + 1))) ;
         }
-    }
-
+    }    
+    
     /** 
      *  Cache data for a slot.
      *
@@ -254,8 +183,8 @@ module StateTransition {
      *
      *  @todo       Make this a method to have a def closer to Eth2 implementation.  
      */
-    method processSlot(s: BeaconState) returns (s' : BeaconState)
-        requires s.slot as nat + 1 < 0x10000000000000000 as nat
+    method {:fuel wellTypedContainer,3} {:fuel getHashTreeRootBytes32,0,0} processSlot(s: BeaconState) returns (s' : BeaconState)   
+        requires s.slot.n as nat + 1 < 0x10000000000000000 as nat
 
         ensures  s.latest_block_header.state_root == EMPTY_BYTES32 ==>
             s' == resolveStateRoot(s).(slot := s.slot)
@@ -267,19 +196,19 @@ module StateTransition {
 
         //  Cache state root
         //  Record the hash of the previous state in the history.
-        var previous_state_root := hash_tree_root(s); 
+        var previous_state_root := getHashTreeRootBytes32(s); 
 
-        s' := s'.(state_roots := s'.state_roots[(s'.slot % SLOTS_PER_HISTORICAL_ROOT) as int := previous_state_root]);
+        s' := castToBeaconState(s'.(state_roots :=  Vector(s'.state_roots.v[(s'.slot.n % SLOTS_PER_HISTORICAL_ROOT as nat) as int := previous_state_root])));
 
         //  Cache latest block header state root
         if (s'.latest_block_header.state_root == EMPTY_BYTES32) {
-            s' := s'.(latest_block_header := s'.latest_block_header.(state_root := previous_state_root));
+            s' := castToBeaconState(s'.(latest_block_header := s'.latest_block_header.(state_root := previous_state_root)));
         }
 
         //  Cache block root
-        var previous_block_root := hash_tree_root(s'.latest_block_header);
+        var previous_block_root := getHashTreeRootBytes32(s'.latest_block_header);
 
-        s' := s'.(block_roots := s'.block_roots[(s.slot % SLOTS_PER_HISTORICAL_ROOT) as int := previous_block_root]);
+        s' := castToBeaconState(s'.(block_roots := Vector(s'.block_roots.v[(s.slot.n % SLOTS_PER_HISTORICAL_ROOT as nat) as int := previous_block_root])));
     }
 
     /**
@@ -289,7 +218,7 @@ module StateTransition {
      */
     method processBlock(s: BeaconState, b: BeaconBlockHeader) returns (s' : BeaconState) 
         requires b.slot == s.slot
-        requires b.parent_root == hash_tree_root(s.latest_block_header)
+        requires b.parent_root == getHashTreeRootBytes32(s.latest_block_header)
 
         ensures s' == addBlockToState(s, b)
 
@@ -308,19 +237,22 @@ module StateTransition {
      *
      *  @note   Matches eth2.0 specs except proposer slashing verification
      */
-    method processBlockHeader(s: BeaconState, b: BeaconBlockHeader) returns (s' : BeaconState) 
+    method {:fuel wellTypedContainer,3} processBlockHeader(s: BeaconState, b: BeaconBlockHeader) returns (s' : BeaconState) 
         //  Verify that the slots match
         requires b.slot == s.slot  
         // Verify that the parent matches
-        requires b.parent_root == hash_tree_root(s.latest_block_header) 
+        requires b.parent_root == getHashTreeRootBytes32(s.latest_block_header) 
 
         ensures s' == addBlockToState(s, b)
     {
-        s':= s.(
-            latest_block_header := BeaconBlockHeader(
-                b.slot,
-                b.parent_root,
-                EMPTY_BYTES32
+        s' :=
+        castToBeaconState(
+                s.(
+                latest_block_header := BeaconBlockHeader(
+                    b.slot,
+                    b.parent_root,
+                    EMPTY_BYTES32
+                )
             )
         );
     }
@@ -334,17 +266,19 @@ module StateTransition {
      *  @param  b   A block to add to the state `s`.
      *  @returns    The state `s` updated to point to `b` with state_root set to 0.
      */
-    function addBlockToState(s: BeaconState, b: BeaconBlockHeader) :  BeaconState 
+    function {:fuel wellTypedContainer,3} addBlockToState(s: BeaconState, b: BeaconBlockHeader) :  BeaconState 
         //  Verify that the slots match
         requires b.slot == s.slot  
         // Verify that the parent matches
-        requires b.parent_root == hash_tree_root(s.latest_block_header) 
+        requires b.parent_root == getHashTreeRootBytes32(s.latest_block_header) 
     {
-        s.(
-            latest_block_header := BeaconBlockHeader(
-                b.slot,
-                b.parent_root,
-                EMPTY_BYTES32
+        castToBeaconState(
+            s.(
+                latest_block_header := BeaconBlockHeader(
+                    b.slot,
+                    b.parent_root,
+                    EMPTY_BYTES32
+                )
             )
         )
     }
@@ -354,32 +288,37 @@ module StateTransition {
      *
      *  @param  s   A beacon state.
      *  @returns    A new state `s' such that:
-     *              1. a new latest_block_header' state_root set to the hash_tree_root(s) 
-     *              2. the hash_tree_root(s) archived in the s'.state_roots for the slot
-     *              3. the hash_tree_root of the new_block_header is archived 
+     *              1. a new latest_block_header' state_root set to the getHashTreeRootBytes32(s) 
+     *              2. the getHashTreeRootBytes32(s) archived in the s'.state_roots for the slot
+     *              3. the getHashTreeRootBytes32 of the new_block_header is archived 
      *              in s'.block_roots
      */
-    function resolveStateRoot(s: BeaconState): BeaconState 
+    function {:fuel wellTypedContainer,3} {:fuel getHashTreeRootBytes32,0,0} resolveStateRoot(s: BeaconState): BeaconState 
         //  Make sure s.slot does not  overflow
-        requires s.slot as nat + 1 < 0x10000000000000000 as nat
+        // requires wellTyped(s)
+        requires s.slot.n as nat + 1 < 0x10000000000000000 as nat
         //  parent_root of the state block header is preserved
         ensures s.latest_block_header.parent_root == resolveStateRoot(s).latest_block_header.parent_root
     {
         var new_latest_block_header := 
             if (s.latest_block_header.state_root == EMPTY_BYTES32 ) then 
-                s.latest_block_header.(state_root := hash_tree_root(s))
+                s.latest_block_header.(state_root := getHashTreeRootBytes32(s))
             else 
                 s.latest_block_header
             ;
+
+        assert wellTypedContainer(new_latest_block_header);
         
-        BeaconState(
-            // slot unchanged
-            s.slot + 1,
-            new_latest_block_header,
-            //  add new block_header root to block_roots history.
-            s.block_roots[(s.slot % SLOTS_PER_HISTORICAL_ROOT) as int := hash_tree_root(new_latest_block_header)],
-            //  add previous state root to state_roots history
-            s.state_roots[(s.slot % SLOTS_PER_HISTORICAL_ROOT) as int := hash_tree_root(s)]
+        castToBeaconState(
+            BeaconState(
+                // slot unchanged
+                Uint64(s.slot.n + 1),
+                new_latest_block_header,
+                //  add new block_header root to block_roots history.
+                Vector(s.block_roots.v[(s.slot.n % SLOTS_PER_HISTORICAL_ROOT as nat) as int := getHashTreeRootBytes32(new_latest_block_header)]),
+                //  add previous state root to state_roots history
+                Vector(s.state_roots.v[(s.slot.n % SLOTS_PER_HISTORICAL_ROOT as nat) as int := getHashTreeRootBytes32(s)])
+            )
         )
     }
 
@@ -391,16 +330,16 @@ module StateTransition {
      *  @returns        A new state obtained by  archiving roots and incrementing slot.
      *                  slot.
      */
-    function forwardStateToSlot(s: BeaconState, slot: Slot) : BeaconState 
-        requires s.slot <= slot
+    function {:fuel wellTypedContainer,2} forwardStateToSlot(s: BeaconState, slot: Slot) : BeaconState 
+        requires s.slot.n <= slot as nat
 
-        ensures forwardStateToSlot(s, slot).slot == slot
+        ensures forwardStateToSlot(s, slot).slot.n == slot as nat
         ensures forwardStateToSlot(s, slot).latest_block_header ==  s.latest_block_header
 
         //  termination ranking function
-        decreases slot - s.slot
+        decreases slot as nat - s.slot.n
     {
-        if (s.slot == slot) then 
+        if (s.slot.n == slot as nat) then 
             s
         else
             nextSlot(forwardStateToSlot(s, slot - 1))
@@ -416,19 +355,21 @@ module StateTransition {
      *              the previous state_root and block_root, and copy verbatim the 
      *              latest_block_header.
      */
-    function nextSlot(s : BeaconState) : BeaconState 
+    function {:fuel wellTypedContainer,3} nextSlot(s : BeaconState) : BeaconState 
         //  Make sure s.slot does not overflow
-        requires s.slot as nat + 1 < 0x10000000000000000 as nat
+        requires s.slot.n as nat + 1 < 0x10000000000000000 as nat
     {
         //  Add header root to history of block_roots
-        var new_block_roots := s.block_roots[(s.slot % SLOTS_PER_HISTORICAL_ROOT) as int := hash_tree_root(s.latest_block_header)];
+        var new_block_roots := s.block_roots.v[(s.slot.n % SLOTS_PER_HISTORICAL_ROOT as nat) as int := getHashTreeRootBytes32(s.latest_block_header)];
         //  Add state root to history of state roots
-        var new_state_roots := s.state_roots[(s.slot % SLOTS_PER_HISTORICAL_ROOT) as int := hash_tree_root(s)];
+        var new_state_roots := s.state_roots.v[(s.slot.n % SLOTS_PER_HISTORICAL_ROOT as nat) as int := getHashTreeRootBytes32(s)];
         //  Increment slot and copy latest_block_header
-        s.(
-            slot := s.slot + 1,
-            block_roots := new_block_roots,
-            state_roots := new_state_roots
+        castToBeaconState(
+            s.(
+                slot := Uint64(s.slot.n + 1),
+                block_roots := Vector(new_block_roots),
+                state_roots := Vector(new_state_roots)
+            )
         )
     }
 }
