src/dafny/beacon/BeaconConstants.dfy
@@ -1,0 +1,52 @@
+/*
+ * Copyright 2020 ConsenSys AG.
+ *
+ * Licensed under the Apache License, Version 2.0 (the "License"); you may 
+ * not use this file except in compliance with the License. You may obtain 
+ * a copy of the License at http://www.apache.org/licenses/LICENSE-2.0
+ *
+ * Unless required by applicable law or agreed to in writing, software dis-
+ * tributed under the License is distributed on an "AS IS" BASIS, WITHOUT 
+ * WARRANTIES OR CONDITIONS OF ANY KIND, either express or implied. See the 
+ * License for the specific language governing permissions and limitations 
+ * under the License.
+ */
+ 
+include "../utils/Eth2Types.dfy"
+include "../utils/Helpers.dfy"
+include "../ssz/Constants.dfy"
+include "../merkle/Merkleise.dfy"
+include "../ssz/Eth2TypeDependentConstants.dfy"
+
+module BeaconConstants {
+    import opened Eth2Types
+    import opened Helpers
+    import opened Constants
+    import opened SSZ_Merkleise
+    import opened Eth2TypeDependentConstants
+
+    /** The historical roots type.  */
+    const EMPTY_HIST_ROOTS := Vector(timeSeq<Bytes32>(EMPTY_BYTES32, SLOTS_PER_HISTORICAL_ROOT as int))
+
+    const EMPTY_BLOCK_HEADER: Serialisable := BeaconBlockHeader(Uint64(0), EMPTY_BYTES32, EMPTY_BYTES32)
+    
+    /**
+     *  Genesis (initial) beacon state.
+     *  
+     *  @link{https://github.com/ethereum/eth2.0-specs/blob/dev/specs/phase0/beacon-chain.md#genesis-state}
+     */
+    const GENESIS_STATE: BeaconState := BeaconState(Uint64(0), EMPTY_BLOCK_HEADER, EMPTY_HIST_ROOTS, EMPTY_HIST_ROOTS)
+
+    /**
+     *  Genesis block (header).
+     *
+     *  @link{https://github.com/ethereum/eth2.0-specs/blob/dev/specs/phase0/beacon-chain.md#genesis-block}
+     *  @note   In this simplified version blocks are same as headers.
+     */
+    const GENESIS_BLOCK_HEADER: BeaconBlockHeader := BeaconBlockHeader(
+        Uint64(0),  
+        EMPTY_BYTES32 , 
+        getHashTreeRootBytes32(GENESIS_STATE)
+    )
+
+}
