src/dafny/ssz/Constants.dfy
@@ -9,8 +9,6 @@ include "../utils/Eth2Types.dfy"
 module Constants {  
   import opened NativeTypes
 
-  import opened Eth2Types
-
   //  Powers of 2
   const TWO_UP_0 := 1;
   const TWO_UP_2 := 2 * TWO_UP_0;
@@ -125,14 +123,5 @@ module Constants {
 
   /** A 0 byte, all bits set to false. */
   const FALSE_BYTE := [false, false, false, false, false, false, false, false]
-  
-  /** An empty chunk, all 32 bytes set to zero */
-  const EMPTY_CHUNK:seq<byte> := [0, 0, 0, 0,
-                                  0, 0, 0, 0,
-                                  0, 0, 0, 0,
-                                  0, 0, 0, 0,
-                                  0, 0, 0, 0,
-                                  0, 0, 0, 0,
-                                  0, 0, 0, 0,
-                                  0, 0, 0, 0]
+
 } 
