src/dafny/ssz/Eth2TypeDependentConstants.dfy
@@ -1,0 +1,39 @@
+/*
+ * Copyright 2020 ConsenSys AG.
+ *
+ * Licensed under the Apache License, Version 2.0 (the "License"); you may 
+ * not use this file except in compliance with the License. You may obtain 
+ * a copy of the License at http://www.apache.org/licenses/LICENSE-2.0
+ *
+ * Unless required by applicable law or agreed to in writing, software dis-
+ * tributed under the License is distributed on an "AS IS" BASIS, WITHOUT 
+ * WARRANTIES OR CONDITIONS OF ANY KIND, either express or implied. See the 
+ * License for the specific language governing permissions and limitations 
+ * under the License.
+ */
+
+include "../utils/Eth2Types.dfy"
+include "../utils/Helpers.dfy"
+
+module Eth2TypeDependentConstants {
+    import opened Eth2Types
+    import opened Helpers
+
+  /** An empty chunk, all 32 bytes set to zero */
+  const EMPTY_CHUNK:seq<byte> := [0, 0, 0, 0,
+                                  0, 0, 0, 0,
+                                  0, 0, 0, 0,
+                                  0, 0, 0, 0,
+                                  0, 0, 0, 0,
+                                  0, 0, 0, 0,
+                                  0, 0, 0, 0,
+                                  0, 0, 0, 0]
+
+    /** The default zeroed Bytes32.  */
+  const SEQ_EMPTY_32_BYTES := timeSeq<byte>(0,32)   
+
+  /**
+    *  The default (empty) Bytes32
+    */
+  const EMPTY_BYTES32 : Bytes32 := Bytes(SEQ_EMPTY_32_BYTES)
+}
